<?xml version="1.0"?>
<rdf:RDF xmlns="https://w3id.org/hdgi/gesture-interaction-pattern"
     xml:base="https://w3id.org/hdgi/gesture-interaction-pattern"
     xmlns:dc="http://purl.org/dc/elements/1.1/"
     xmlns:ns="http://creativecommons.org/ns#"
     xmlns:owl="http://www.w3.org/2002/07/owl#"
     xmlns:rdf="http://www.w3.org/1999/02/22-rdf-syntax-ns#"
     xmlns:xml="http://www.w3.org/XML/1998/namespace"
     xmlns:xsd="http://www.w3.org/2001/XMLSchema#"
     xmlns:prov="http://www.w3.org/ns/prov#"
     xmlns:rdfs="http://www.w3.org/2000/01/rdf-schema#"
     xmlns:time="https://www.w3.org/TR/owl-time/#time:"
     xmlns:skos1="http://www.w3.org/2008/05/skos#"
     xmlns:terms="http://purl.org/dc/terms/"
     xmlns:cpannotationschema="http://www.ontologydesignpatterns.org/schemas/cpannotationschema.owl#">
    <owl:Ontology rdf:about="https://w3id.org/hdgi/gesture-interaction-pattern">
        <owl:imports rdf:resource="http://www.ontologydesignpatterns.org/schemas/cpannotationschema.owl"/>
        <ns:attributionURL xml:lang="en">https://w3id.org/hdgi/gesture-interaction-pattern</ns:attributionURL>
        <dc:creator xml:lang="en">Madhawa Perera, Armin Haller</dc:creator>
        <terms:description xml:lang="en">Ontology pattern to model concepts related to human gesture interactions.</terms:description>
        <terms:license rdf:resource="https://github.com/madhawap/human-device-gesture-interaction-ontology/blob/master/LICENSE"/>
        <terms:title xml:lang="en">Gesture Interaction Pattern: a content ontology design pattern.</terms:title>
        <cpannotationschema:extractedFrom rdf:resource="https://w3id.org/hdgi/v0.1"/>
        <cpannotationschema:hasIntent xml:lang="en">The Gesture Interaction Pattern aims to model the pose and movement of human body that are used to interact with devices (particularly with device affordances). This helps to describe a human gesture with its relationship between certain device affordances, related body parts and the temporal components associated with those.

This might be helpful in creating user specific gesture profiles. This ontology pattern is geared at mapping the ubiquitousness in gesture vocabularies by linking them appropriately and does not enforce designers and manufacturers to follow a standard.</cpannotationschema:hasIntent>
        <cpannotationschema:scenarios xml:lang="en">This pattern is applicable for a wide range of scenarios in gesture interaction systems.

For example:

Consider a user who uses a certain gesture to turn on their personal air conditioner. If this user visits a hotel room with an air conditioner of a different model that carries different interactions, how can the system accommodate the user&apos;s preferred gesture and let the user continue, as in their own room, without having to read instructions. This ontology pattern will help to model parsonlised gesture details.

Further, online search engines currently do not provide sufficient information for gesture related semantics. For example, search query to retrieve ‘gestures to turn on a TV’, would not provide relevant gesture vocabularies supported by different vendors. Designers/developers have to find individual studies separately and read/learn necessary data manually.  Being able to retrieve semantics of gestures which are related to the affordance of ‘turn on a TV’ would be convenient for designers and developers in such situations.</cpannotationschema:scenarios>
        <rdfs:label xml:lang="en">Gesture Interaction Pattern</rdfs:label>
        <rdfs:seeAlso xml:lang="en">Refer to https://w3id.org/hdgi to see a complete ontology schema build around Gesture Interaction Pattern</rdfs:seeAlso>
    </owl:Ontology>
    


    <!-- 
    ///////////////////////////////////////////////////////////////////////////////////////
    //
    // Annotation properties
    //
    ///////////////////////////////////////////////////////////////////////////////////////
     -->

    


    <!-- http://creativecommons.org/ns#attributionURL -->

    <owl:AnnotationProperty rdf:about="http://creativecommons.org/ns#attributionURL">
        <dc:creator>madhawaperera</dc:creator>
    </owl:AnnotationProperty>
    


    <!-- http://purl.org/dc/elements/1.1/creator -->

    <owl:AnnotationProperty rdf:about="http://purl.org/dc/elements/1.1/creator">
        <dc:creator>madhawaperera</dc:creator>
    </owl:AnnotationProperty>
    


    <!-- http://purl.org/dc/terms/description -->

    <owl:AnnotationProperty rdf:about="http://purl.org/dc/terms/description">
        <dc:creator>madhawaperera</dc:creator>
    </owl:AnnotationProperty>
    


    <!-- http://purl.org/dc/terms/license -->

    <owl:AnnotationProperty rdf:about="http://purl.org/dc/terms/license">
        <dc:creator>madhawaperera</dc:creator>
    </owl:AnnotationProperty>
    


    <!-- http://purl.org/dc/terms/title -->

    <owl:AnnotationProperty rdf:about="http://purl.org/dc/terms/title">
        <dc:creator>madhawaperera</dc:creator>
    </owl:AnnotationProperty>
    


    <!-- http://www.w3.org/2008/05/skos#example -->

    <owl:AnnotationProperty rdf:about="http://www.w3.org/2008/05/skos#example">
        <dc:creator>madhawaperera</dc:creator>
    </owl:AnnotationProperty>
    


    <!-- 
    ///////////////////////////////////////////////////////////////////////////////////////
    //
    // Object Properties
    //
    ///////////////////////////////////////////////////////////////////////////////////////
     -->

    


    <!-- https://w3id.org/hdgi/gesture-interaction-pattern1affordedBy -->

    <owl:ObjectProperty rdf:about="https://w3id.org/hdgi/gesture-interaction-pattern1affordedBy">
        <rdfs:comment xml:lang="en">Relation between an Affordance and the Device classes where a device is able to afford it.</rdfs:comment>
        <rdfs:label xml:lang="en">affordedBy</rdfs:label>
        <skos1:example xml:lang="en">Turn on TV</skos1:example>
    </owl:ObjectProperty>
    


    <!-- https://w3id.org/hdgi/gesture-interaction-pattern1hasDuration -->

    <owl:ObjectProperty rdf:about="https://w3id.org/hdgi/gesture-interaction-pattern1hasDuration">
        <rdfs:comment xml:lang="en">Relation between a Gesture and the Duration, where the gesture has a duration. This is an owl:equivalentClass time:hasDuration.</rdfs:comment>
        <rdfs:label xml:lang="en">hasDuration</rdfs:label>
    </owl:ObjectProperty>
    


    <!-- https://w3id.org/hdgi/gesture-interaction-pattern1hasEndPose -->

    <owl:ObjectProperty rdf:about="https://w3id.org/hdgi/gesture-interaction-pattern1hasEndPose">
        <rdfs:comment xml:lang="en">Relation between a Gesture and a Pose where the pose represents the ending Pose of that gesture.</rdfs:comment>
        <rdfs:label xml:lang="en">hasEndPose</rdfs:label>
    </owl:ObjectProperty>
    


    <!-- https://w3id.org/hdgi/gesture-interaction-pattern1hasMovement -->

    <owl:ObjectProperty rdf:about="https://w3id.org/hdgi/gesture-interaction-pattern1hasMovement">
        <rdfs:comment xml:lang="en">Relation between a Gesture and a Movement where the movement describes a particular motion of a body part.</rdfs:comment>
        <rdfs:label xml:lang="en">hasMovement</rdfs:label>
    </owl:ObjectProperty>
    


    <!-- https://w3id.org/hdgi/gesture-interaction-pattern1hasStartPose -->

    <owl:ObjectProperty rdf:about="https://w3id.org/hdgi/gesture-interaction-pattern1hasStartPose">
        <rdfs:comment xml:lang="en">Relation between a Gesture and Pose where the pose represents the initial pose of that gesture.</rdfs:comment>
        <rdfs:label xml:lang="en">hasStartPose</rdfs:label>
    </owl:ObjectProperty>
    


    <!-- https://w3id.org/hdgi/gesture-interaction-pattern1includesGesture -->

    <owl:ObjectProperty rdf:about="https://w3id.org/hdgi/gesture-interaction-pattern1includesGesture">
        <rdfs:comment xml:lang="en">A Gesture could consist multiple atomic Gestures. This represents the relation between the Gesture and its atomic Gestures.</rdfs:comment>
        <rdfs:label xml:lang="en">includesGestures</rdfs:label>
    </owl:ObjectProperty>
    


    <!-- https://w3id.org/hdgi/gesture-interaction-pattern1performs -->

    <owl:ObjectProperty rdf:about="https://w3id.org/hdgi/gesture-interaction-pattern1performs">
        <rdfs:comment xml:lang="en">Relation between a Human and a Gesture.</rdfs:comment>
        <rdfs:label xml:lang="en">performs</rdfs:label>
    </owl:ObjectProperty>
    


    <!-- https://w3id.org/hdgi/gesture-interaction-pattern1supportsGesture -->

    <owl:ObjectProperty rdf:about="https://w3id.org/hdgi/gesture-interaction-pattern1supportsGesture">
        <rdfs:comment xml:lang="en">Relation between a Gesture and an Affordance where affordance is supported by that particular gesture.</rdfs:comment>
        <rdfs:label xml:lang="en">supportsGesture</rdfs:label>
    </owl:ObjectProperty>
    


    <!-- https://w3id.org/hdgi/gesture-interaction-pattern1used -->

    <owl:ObjectProperty rdf:about="https://w3id.org/hdgi/gesture-interaction-pattern1used">
        <rdfs:comment xml:lang="en">Relation between a Gesture and a BodyPart which describes the body parts used in that gesture. This is an owl:equivalentClass prov:used.</rdfs:comment>
        <rdfs:label xml:lang="en">used</rdfs:label>
    </owl:ObjectProperty>
    


    <!-- https://w3id.org/hdgi/gesture-interaction-pattern1uses -->

    <owl:ObjectProperty rdf:about="https://w3id.org/hdgi/gesture-interaction-pattern1uses">
        <rdfs:comment xml:lang="en">Relation between a Human and BodyPart which describes the body part that a human uses to perform a certain gesture.</rdfs:comment>
        <rdfs:label xml:lang="en">uses</rdfs:label>
    </owl:ObjectProperty>
    


    <!-- 
    ///////////////////////////////////////////////////////////////////////////////////////
    //
    // Data properties
    //
    ///////////////////////////////////////////////////////////////////////////////////////
     -->

    


    <!-- https://w3id.org/hdgi/gesture-interaction-pattern1timestamp -->

    <owl:DatatypeProperty rdf:about="https://w3id.org/hdgi/gesture-interaction-pattern1timestamp">
        <rdfs:range rdf:resource="http://www.w3.org/2001/XMLSchema#dateTimeStamp"/>
        <rdfs:comment xml:lang="en">A timestamp represent the date and time of an event occured and that is recorded by a system/person.</rdfs:comment>
        <rdfs:label xml:lang="en">timestamp</rdfs:label>
    </owl:DatatypeProperty>
    


    <!-- 
    ///////////////////////////////////////////////////////////////////////////////////////
    //
    // Classes
    //
    ///////////////////////////////////////////////////////////////////////////////////////
     -->

    


    <!-- https://w3id.org/hdgi/gesture-interaction-pattern1Affordance -->

    <owl:Class rdf:about="https://w3id.org/hdgi/gesture-interaction-pattern1Affordance">
        <rdfs:subClassOf>
            <owl:Restriction>
                <owl:onProperty rdf:resource="https://w3id.org/hdgi/gesture-interaction-pattern1affordedBy"/>
                <owl:allValuesFrom rdf:resource="https://w3id.org/hdgi/gesture-interaction-pattern1Device"/>
            </owl:Restriction>
        </rdfs:subClassOf>
        <rdfs:subClassOf>
            <owl:Restriction>
                <owl:onProperty rdf:resource="https://w3id.org/hdgi/gesture-interaction-pattern1supportsGesture"/>
                <owl:allValuesFrom rdf:resource="https://w3id.org/hdgi/gesture-interaction-pattern1Gesture"/>
            </owl:Restriction>
        </rdfs:subClassOf>
        <rdfs:comment xml:lang="en">Affordance is a quality or characteristic of Devices that indicates the possible action a Human can take with it. This is rdfs:subClassOf ssn:Property.</rdfs:comment>
        <rdfs:label xml:lang="en">Affordance</rdfs:label>
    </owl:Class>
    


    <!-- https://w3id.org/hdgi/gesture-interaction-pattern1BodyPart -->

    <owl:Class rdf:about="https://w3id.org/hdgi/gesture-interaction-pattern1BodyPart">
        <rdfs:comment xml:lang="en">BodyPart is any part of HumanBody such as an Face, Leg etc.</rdfs:comment>
        <rdfs:label xml:lang="en">BodyPart</rdfs:label>
    </owl:Class>
    


    <!-- https://w3id.org/hdgi/gesture-interaction-pattern1Device -->

    <owl:Class rdf:about="https://w3id.org/hdgi/gesture-interaction-pattern1Device">
        <rdfs:comment xml:lang="en">Device denotes a piece of hardware or software which consists of sensors or actuators or both.</rdfs:comment>
        <rdfs:label xml:lang="en">Device</rdfs:label>
    </owl:Class>
    


    <!-- https://w3id.org/hdgi/gesture-interaction-pattern1Duration -->

    <owl:Class rdf:about="https://w3id.org/hdgi/gesture-interaction-pattern1Duration">
        <rdfs:comment xml:lang="en">Duration of a temporal extent expressed as a decimal number scaled by a temporal unit. This is an owl:equivalentClass time:Duration.</rdfs:comment>
        <rdfs:label xml:lang="en">Duration</rdfs:label>
    </owl:Class>
    


    <!-- https://w3id.org/hdgi/gesture-interaction-pattern1Gesture -->

    <owl:Class rdf:about="https://w3id.org/hdgi/gesture-interaction-pattern1Gesture">
        <rdfs:subClassOf>
            <owl:Restriction>
                <owl:onProperty rdf:resource="https://w3id.org/hdgi/gesture-interaction-pattern1includesGesture"/>
                <owl:allValuesFrom rdf:resource="https://w3id.org/hdgi/gesture-interaction-pattern1Gesture"/>
            </owl:Restriction>
        </rdfs:subClassOf>
        <rdfs:subClassOf>
            <owl:Restriction>
                <owl:onProperty rdf:resource="https://w3id.org/hdgi/gesture-interaction-pattern1used"/>
                <owl:allValuesFrom rdf:resource="https://w3id.org/hdgi/gesture-interaction-pattern1BodyPart"/>
            </owl:Restriction>
        </rdfs:subClassOf>
        <rdfs:subClassOf>
            <owl:Restriction>
                <owl:onProperty rdf:resource="https://w3id.org/hdgi/gesture-interaction-pattern1hasEndPose"/>
                <owl:qualifiedCardinality rdf:datatype="http://www.w3.org/2001/XMLSchema#nonNegativeInteger">1</owl:qualifiedCardinality>
                <owl:onClass rdf:resource="https://w3id.org/hdgi/gesture-interaction-pattern1Pose"/>
            </owl:Restriction>
        </rdfs:subClassOf>
        <rdfs:subClassOf>
            <owl:Restriction>
                <owl:onProperty rdf:resource="https://w3id.org/hdgi/gesture-interaction-pattern1hasStartPose"/>
                <owl:qualifiedCardinality rdf:datatype="http://www.w3.org/2001/XMLSchema#nonNegativeInteger">1</owl:qualifiedCardinality>
                <owl:onClass rdf:resource="https://w3id.org/hdgi/gesture-interaction-pattern1Pose"/>
            </owl:Restriction>
        </rdfs:subClassOf>
        <rdfs:subClassOf>
            <owl:Restriction>
                <owl:onProperty rdf:resource="https://w3id.org/hdgi/gesture-interaction-pattern1hasMovement"/>
                <owl:maxQualifiedCardinality rdf:datatype="http://www.w3.org/2001/XMLSchema#nonNegativeInteger">1</owl:maxQualifiedCardinality>
                <owl:onClass rdf:resource="https://w3id.org/hdgi/gesture-interaction-pattern1Movement"/>
            </owl:Restriction>
        </rdfs:subClassOf>
        <rdfs:comment xml:lang="en">Gesture is a Movement or a Pose of a BodyPart.</rdfs:comment>
        <rdfs:label xml:lang="en">Gesture</rdfs:label>
    </owl:Class>
    


    <!-- https://w3id.org/hdgi/gesture-interaction-pattern1Human -->

    <owl:Class rdf:about="https://w3id.org/hdgi/gesture-interaction-pattern1Human">
        <rdfs:subClassOf>
            <owl:Restriction>
                <owl:onProperty rdf:resource="https://w3id.org/hdgi/gesture-interaction-pattern1performs"/>
                <owl:someValuesFrom rdf:resource="https://w3id.org/hdgi/gesture-interaction-pattern1Gesture"/>
            </owl:Restriction>
        </rdfs:subClassOf>
        <rdfs:subClassOf>
            <owl:Restriction>
                <owl:onProperty rdf:resource="https://w3id.org/hdgi/gesture-interaction-pattern1performs"/>
                <owl:someValuesFrom rdf:resource="https://w3id.org/hdgi/gesture-interaction-pattern1Pose"/>
            </owl:Restriction>
        </rdfs:subClassOf>
        <rdfs:subClassOf>
            <owl:Restriction>
                <owl:onProperty rdf:resource="https://w3id.org/hdgi/gesture-interaction-pattern1uses"/>
                <owl:allValuesFrom rdf:resource="https://w3id.org/hdgi/gesture-interaction-pattern1BodyPart"/>
            </owl:Restriction>
        </rdfs:subClassOf>
        <rdfs:comment xml:lang="en">Human represents the user who performs a Gesture or a Pose.</rdfs:comment>
        <rdfs:label xml:lang="en">Human</rdfs:label>
    </owl:Class>
    


    <!-- https://w3id.org/hdgi/gesture-interaction-pattern1Movement -->

    <owl:Class rdf:about="https://w3id.org/hdgi/gesture-interaction-pattern1Movement">
        <rdfs:subClassOf>
            <owl:Restriction>
                <owl:onProperty rdf:resource="https://w3id.org/hdgi/gesture-interaction-pattern1hasDuration"/>
                <owl:qualifiedCardinality rdf:datatype="http://www.w3.org/2001/XMLSchema#nonNegativeInteger">1</owl:qualifiedCardinality>
                <owl:onClass rdf:resource="https://w3id.org/hdgi/gesture-interaction-pattern1Duration"/>
            </owl:Restriction>
        </rdfs:subClassOf>
        <rdfs:comment xml:lang="en">Movement is the act of moving a certain BodyPart towards a certain direction in a certain period of time (Duration).</rdfs:comment>
        <rdfs:label xml:lang="en">Movement</rdfs:label>
    </owl:Class>
    


    <!-- https://w3id.org/hdgi/gesture-interaction-pattern1Pose -->

    <owl:Class rdf:about="https://w3id.org/hdgi/gesture-interaction-pattern1Pose">
        <rdfs:subClassOf>
            <owl:Restriction>
                <owl:onProperty rdf:resource="https://w3id.org/hdgi/gesture-interaction-pattern1timestamp"/>
                <owl:qualifiedCardinality rdf:datatype="http://www.w3.org/2001/XMLSchema#nonNegativeInteger">1</owl:qualifiedCardinality>
                <owl:onDataRange rdf:resource="http://www.w3.org/2001/XMLSchema#dateTimeStamp"/>
            </owl:Restriction>
        </rdfs:subClassOf>
        <rdfs:comment xml:lang="en">Pose is repesent a particular Position and Rotation of a BodyPart at a particular timestamp.</rdfs:comment>
        <rdfs:label xml:lang="en">Pose</rdfs:label>
    </owl:Class>
</rdf:RDF>



<!-- Generated by the OWL API (version 4.5.9.2019-02-01T07:24:44Z) https://github.com/owlcs/owlapi -->

